SStructTT/SStruct/Erasure/Normalize.lean
@@ -9,25 +9,25 @@ lemma Erased.value_step {m n : Tm Srt} :
     Value m -> m ~>> n -> False := by
   intro vl st; induction vl generalizing n
   case lam =>
-    rcases st with ⟨rd, st⟩
+    rcases st with ⟨_, rd, st⟩
     rw[rd.lam_inv] at st; cases st
   case tup ihm ihn =>
-    rcases st with ⟨rd, st⟩
+    rcases st with ⟨_, rd, st⟩
     have ⟨_, _, _, rd1, rd2⟩ := rd.tup_inv
     subst_vars; cases st
-    case tup_M st => apply ihm (Step.intro rd1 st)
-    case tup_N st => apply ihn (Step.intro rd2 st)
+    case tup_M st => apply ihm ⟨_, rd1, st⟩
+    case tup_N st => apply ihn ⟨_, rd2, st⟩
   case tt =>
-    rcases st with ⟨rd, st⟩
+    rcases st with ⟨_, rd, st⟩
     rw[rd.tt_inv] at st; cases st
   case ff =>
-    rcases st with ⟨rd, st⟩
+    rcases st with ⟨_, rd, st⟩
     rw[rd.ff_inv] at st; cases st
   case ptr =>
-    rcases st with ⟨rd, st⟩
+    rcases st with ⟨_, rd, st⟩
     rw[rd.ptr_inv] at st; cases st
   case null =>
-    rcases st with ⟨rd, st⟩
+    rcases st with ⟨_, rd, st⟩
     rw[rd.null_inv] at st; cases st
 
 variable [ord : SrtOrder Srt]
